Engine: add oracles to all definitions

Engine/Correctness.v
@@ -42,18 +42,18 @@ Section Correctness.
   Context (rer: RegExpRecord).
 
 Definition trc_pike_tree := @trc pike_tree_state pike_tree_step.
-Definition trc_pike_vm (c:code) (dir:Direction) := @trc pike_vm_state (pike_vm_step rer c dir).
+Definition trc_pike_vm (c:code) (dir:Direction) (os:nfa_oracles) := @trc pike_vm_state (pike_vm_step rer c dir os).
 
 (* The Pike invariant is preserved through the TRC *)
 Lemma vm_to_tree:
-  forall svm1 st1 svm2 r code
+  forall svm1 st1 svm2 r code os
     (COMPILE: compilation r = code)
     (STWF: stutter_wf rer code)
-    (INVARIANT: pike_inv rer r st1 svm1)
-    (TRCVM: trc_pike_vm code forward svm1 svm2),
-    exists st2, trc_pike_tree st1 st2 /\ pike_inv rer r st2 svm2.
+    (INVARIANT: pike_inv rer r os st1 svm1)
+    (TRCVM: trc_pike_vm code forward os svm1 svm2),
+    exists st2, trc_pike_tree st1 st2 /\ pike_inv rer r os st2 svm2.
 Proof.
-  intros svm1 st1 svm2 r code COMPILE STWF INVARIANT TRCVM.
+  intros svm1 st1 svm2 r code os COMPILE STWF INVARIANT TRCVM.
   generalize dependent st1. induction TRCVM; intros.
   { exists st1. split; auto. apply trc_refl. }
   eapply PikeEquiv.invariant_preservation in STEP; eauto.
@@ -66,30 +66,30 @@ Qed.
 
 (* Any execution of the PikeVM to a final state corresponds to an execution of the PikeTree *)
 Theorem pike_vm_to_pike_tree:
-  forall r inp tree result,
+  forall r inp os tree result,
     pike_regex r ->
     bool_tree rer [Areg r] inp CanExit forward tree ->
-    trc_pike_vm (compilation r) forward (pike_vm_initial_state inp) (PVS_final result) ->
+    trc_pike_vm (compilation r) forward os (pike_vm_initial_state inp) (PVS_final result) ->
     trc_pike_tree (pike_tree_initial_state tree inp) (PTS_final result).
 Proof.
-  intros r inp tree result SUBSET TREE TRCVM.
-  pose proof (initial_pike_inv rer r inp tree (compilation r) TREE (@eq_refl _ _) SUBSET) as INIT.
+  intros r inp os tree result SUBSET OS TREE TRCVM.
+  pose proof (initial_pike_inv rer r inp os tree TREE SUBSET OS) as INIT.
   eapply vm_to_tree in TRCVM as [vmfinal [TRCTREE INV]]; eauto.
   - inversion INV; subst. auto.
   - eapply compilation_stutter_wf; eauto.
 Qed.
 
 Theorem pike_vm_to_pike_tree_unanchored {strs:StrSearch}:
-  forall r inp tree result future_tree,
+  forall r inp os tree result future_tree,
     pike_regex r ->
     bool_tree rer [Areg r] inp CanExit forward tree ->
-    trc_pike_vm (compilation r) forward (pike_vm_initial_state_unanchored (extract_literal rer r) inp forward) (PVS_final result) ->
+    trc_pike_vm (compilation r) forward os (pike_vm_initial_state_unanchored (extract_literal rer r) inp forward) (PVS_final result) ->
     future_tree_shape rer r inp future_tree ->
     exists future, may_erase future_tree future /\
     trc_pike_tree (pike_tree_initial_state_unanchored tree future inp) (PTS_final result).
 Proof.
-  intros r inp tree result future_tree SUBSET TREE TRCVM NEXTFUTURE.
-  pose proof (initial_pike_inv_unanchored rer _ _ _ _ _ TREE (@eq_refl _ _) SUBSET NEXTFUTURE) as [future [M INIT]].
+  intros r inp os tree result future_tree SUBSET OS TREE TRCVM NEXTFUTURE.
+  pose proof (initial_pike_inv_unanchored rer _ _ _ _ _ TREE SUBSET OS NEXTFUTURE) as [future [M INIT]].
   eapply vm_to_tree in TRCVM as [vmfinal [TRCTREE INV]]; eauto.
   - inversion INV; subst. eauto.
   - eapply compilation_stutter_wf; eauto.
@@ -111,17 +111,17 @@ Qed.
 (** * Correctness Theorem of the PikeVM result  *)
 
 Theorem pike_vm_correct:
-  forall r inp tree result,
+  forall r inp os tree result,
     (* the regex `r` is in the supported subset *)
     pike_regex r ->
     (* `tree` is the tree of the regex `r` for the input `inp` *)
     is_tree rer [Areg r] inp GroupMap.empty forward tree ->
     (* the result of the PikeVM is `result` *)
-    trc_pike_vm (compilation r) forward (pike_vm_initial_state inp) (PVS_final result) ->
+    trc_pike_vm (compilation r) forward os (pike_vm_initial_state inp) (PVS_final result) ->
     (* This `result` is the priority result of the `tree` *)
     result = first_leaf tree inp.
 Proof.
-  intros r inp tree result SUBSET TREE TRC.
+  intros r inp os tree result SUBSET OS TREE TRC.
   eapply encode_equal with (b:=CanExit) in TREE as BOOLTREE; pike_subset.
   eapply pike_vm_to_pike_tree in TRC; eauto.
   assert (SUBTREE: pike_subtree tree).
@@ -133,17 +133,17 @@ Proof.
 Qed.
 
 Theorem pike_vm_correct_unanchored {strs:StrSearch}:
-  forall r inp tree result,
+  forall r inp os tree result,
     (* the regex `r` is in the supported subset *)
     pike_regex r ->
     (* `tree` is the tree of the regex `[^]*?r` for the input `inp` *)
     is_tree rer [Areg (lazy_prefix r)] inp GroupMap.empty forward tree ->
     (* the result of the PikeVM is `result` *)
-    trc_pike_vm (compilation r) forward (pike_vm_initial_state_unanchored (extract_literal rer r) inp forward) (PVS_final result) ->
+    trc_pike_vm (compilation r) forward os (pike_vm_initial_state_unanchored (extract_literal rer r) inp forward) (PVS_final result) ->
     (* This `result` is the priority result of the `tree` *)
     result = first_leaf tree inp.
 Proof.
-  intros r inp tree result SUBSET TREE TRC.
+  intros r inp os tree result SUBSET OS TREE TRC.
   eapply encode_equal with (b:=CanExit) in TREE as BOOLTREE; pike_subset.
   inversion BOOLTREE; inversion CONT; destruct plus; [discriminate|]; subst.
   eapply pike_vm_to_pike_tree_unanchored in TRC as [? [? TRC]]; eauto.
@@ -155,45 +155,45 @@ Qed.
 
 (* Equivalence of PikeVM to Warblre backtracking algorithm *)
 Theorem pike_vm_same_warblre:
-  forall lr wr inp,
+  forall lr los wr inp,
     pike_regex lr ->
     equiv_regex wr lr ->
     RegExpRecord.capturingGroupsCount rer = StaticSemantics.countLeftCapturingParensWithin wr nil ->
     EarlyErrors.Pass_Regex wr nil ->
     forall result,
-      trc_pike_vm (compilation lr) forward (pike_vm_initial_state inp) (PVS_final result) ->
+      trc_pike_vm (compilation lr) forward los (pike_vm_initial_state inp) (PVS_final result) ->
       EquivDef.equiv_res result ((EquivMain.compilePattern wr rer) (input_str inp) (idx inp)).
 Proof.
-  intros lr wr inp Hpike Hequiv Hcapcount HearlyErrors.
+  intros lr los wr inp Hpike Hos Hequiv Hcapcount HearlyErrors.
   pose proof equiv_main wr lr rer inp Hequiv Hcapcount HearlyErrors as HequivMain.
   destruct HequivMain as [m [res [Hcompsucc [Hexecsucc Hsameresult]]]].
   unfold compilePattern. rewrite Hcompsucc, Hexecsucc.
   set (tree := FunctionalUtils.compute_tr rer [Areg lr] inp GroupMap.empty forward).
   specialize (Hsameresult tree eq_refl). destruct Hsameresult as [His_tree Hsameresult].
   intros result Hpikeresult.
-  pose proof pike_vm_correct lr inp tree result Hpike His_tree Hpikeresult as Hsameresult'.
+  pose proof pike_vm_correct lr inp los tree result Hpike Hos His_tree Hpikeresult as Hsameresult'.
   rewrite Hsameresult'. assumption.
 Qed.
 
 (* Same, but with an input that is at the beginning of the input string *)
 Theorem pike_vm_same_warblre_str0:
-  forall lr wr str0,
+  forall lr los wr str0,
     pike_regex lr ->
     equiv_regex wr lr ->
     RegExpRecord.capturingGroupsCount rer = StaticSemantics.countLeftCapturingParensWithin wr nil ->
     EarlyErrors.Pass_Regex wr nil ->
     forall result,
-      trc_pike_vm (compilation lr) forward (pike_vm_initial_state (init_input str0)) (PVS_final result) ->
+      trc_pike_vm (compilation lr) forward los (pike_vm_initial_state (init_input str0)) (PVS_final result) ->
       EquivDef.equiv_res result ((EquivMain.compilePattern wr rer) str0 0).
 Proof.
-  intros lr wr str0 Hpike Hequiv Hcapcount HearlyErrors.
+  intros lr los wr str0 Hpike Hos Hequiv Hcapcount HearlyErrors.
   apply pike_vm_same_warblre; auto.
 Qed.
 
 (* Equivalence of PikeVM to Warblre Semantics *)
 (* A version closer to the paper definition *)
 Theorem pike_vm_warblre:
-  forall rw r inp result,
+  forall rw r os inp result,
     (* For a correct RegExpRecord *)
     RegExpRecord.capturingGroupsCount rer = countLeftCapturingParensWithin rw [] ->
     (* For any Warblre regex that passes the early errors check, *)
@@ -203,11 +203,11 @@ Theorem pike_vm_warblre:
     (* such that it is in the supported PikeVM subset *)
     pike_regex r ->
     (* When PikeVM reaches a final result *)
-    trc_pike_vm (compilation r) forward (pike_vm_initial_state inp) (PVS_final result) ->
+    trc_pike_vm (compilation r) forward os (pike_vm_initial_state inp) (PVS_final result) ->
     (* this result is equal to Warblre's execution result *)
     (compilePattern rw rer) (input_str inp) (idx inp) = to_MatchState result (RegExpRecord.capturingGroupsCount rer).
 Proof.
-  intros rw r inp result RER EARLY TOLINDEN SUBSET TRC.
+  intros rw r os inp result RER EARLY TOLINDEN SUBSET OS TRC.
   specialize (earlyErrors_pass_translation _ EARLY) as [lr SUCCESS].
   unfold warblre_to_linden' in TOLINDEN. rewrite SUCCESS in TOLINDEN. subst.
   specialize (warblre_to_linden_sound_root _ _ SUCCESS) as EQUIV.
@@ -215,7 +215,7 @@ Proof.
   specialize (equiv_main _ _ _ inp EQUIV RER PASS) as [m [res [COMP_SUCC [EXEC_SUCC LW_EQUIV]]]].
   unfold compilePattern. rewrite COMP_SUCC, EXEC_SUCC.
   specialize (LW_EQUIV (compute_tr rer [Areg lr] inp GroupMap.empty forward) eq_refl) as [ISTREE LW_EQUIV].
-  specialize (pike_vm_correct _ _ _ _ SUBSET ISTREE TRC) as FIRST. subst.
+  specialize (pike_vm_correct _ _ _ _ _ SUBSET OS ISTREE TRC) as FIRST. subst.
   symmetry. apply to_MatchState_equal; auto.
   eapply compilePattern_preserves_groupcount; eauto.
 Qed.
